{
 "cells": [
  {
   "cell_type": "markdown",
   "metadata": {},
   "source": [
    "# Homework 0\n",
    "### Jake Pitkin\n",
    "**CS 6190: Probabilistic Modeling - Spring 2018**<br>\n",
    "**January 19th 2018**"
   ]
  },
  {
   "cell_type": "markdown",
   "metadata": {},
   "source": [
    "1. Let $X$ and $Y$ be continuous, real-valued random variables. Prove the following: \n",
    "\n",
    "    (a) $E[[X|Y]] = E[X]$\n",
    "    \n",
    "    First we will use the hint and apply the definition of expectation for continuous random variables over Y.\n",
    "    \n",
    "    $$\\int_{-\\infty}^{\\infty} E[ X | Y ] \\  p_y(y) \\ dy$$\n",
    "    \n",
    "    Next apply the definition of conditional expectation from the lecture notes.\n",
    "    \n",
    "    $$\\int_{-\\infty}^{\\infty} \\int_{-\\infty}^{\\infty} x \\ p_x(x \\ | \\ y) \\ dx \\  p_y(y) \\ dy$$\n",
    "    \n",
    "    Using the definition of joint probability density over two random variables $X, Y$ which is $p(x, y) = p(x|y) * p(y)$.\n",
    "    \n",
    "    $$\\int_{-\\infty}^{\\infty} \\int_{-\\infty}^{\\infty} x \\ p(x,y) \\ dx \\ dy$$\n",
    "    \n",
    "    Now that we have the joint probability density of $X$ and $Y$, we take the marginal density of X from the lecture notes.\n",
    "    \n",
    "    $$\\int_{-\\infty}^{\\infty} x \\ p(x) \\ dx$$\n",
    "    \n",
    "    Finally the definition of expection of a continuous random variable is applied:\n",
    "    \n",
    "    $$\\int_{-\\infty}^{\\infty} x \\ p(x) \\ dx = E[X]$$\n",
    "    \n",
    "    Thus we have shown that $E[[X|Y]] = E[X]$.\n",
    "    <br><br>\n",
    "    \n",
    "    (b) $Var(X) = E[Var(X|Y)] + Var(E[X|Y])$\n",
    "    \n",
    "    For this proof I will be using the expanded definition of variance $Var(x) = E[X^2] - E[X]^2$ which is shown here [wiki](https://en.wikipedia.org/wiki/Variance#Definition).\n",
    "    \n",
    "    Following the hint, we will expand both the terms on the RHS using the above definition of variance. Expanding $E[Var(X|Y)]$:\n",
    "    \n",
    "    $$E[E[X^2|Y] - E[X|Y]^2] + Var(E[X|Y])$$\n",
    "    \n",
    "   And expanding next expanding $Var(E[X|Y])$:\n",
    "   \n",
    "   $$E[E[X^2|Y] - E[X|Y]^2] + E[E[X|Y]^2] - E[E[X|Y]]^2$$\n",
    "   \n",
    "   Next we will use the linearity of expectation from the lecture notes to get two like terms we can cancel out:\n",
    "   \n",
    "   $$E[E[X^2|Y]] - E[E[X|Y]^2] + E[E[X|Y]^2] - E[E[X|Y]]^2$$\n",
    "   \n",
    "   Canceling out like terms:\n",
    "   \n",
    "   $$E[E[X^2|Y]] - E[E[X|Y]]^2$$\n",
    "   \n",
    "   Finally we apply the result from part (a) to both parts of the equation:\n",
    "   \n",
    "   $$E[X^2] - E[X]^2$$\n",
    "   \n",
    "   This matches the expanded definition of $Var(x)$\n",
    "   \n",
    "   $$Var(x) = E[X^2] - E[X]^2$$\n",
    "   \n",
    "   Thus we have shown that $Var(X) = E[Var(X|Y)] + Var(E[X|Y])$. <br><br>\n",
    "   \n",
    "2. Consider random variables $X$ and $Y$ with joint pdf\n",
    "$$\\begin{equation*}\n",
    "p(x, y) =\n",
    "\\begin{cases}\n",
    "x + y \\qquad &\\text{for $0 \\leq x \\leq 1$, and $0 \\leq y \\leq 1$}\\\\\n",
    "0\\qquad &\\text{otherwise}\n",
    "\\end{cases}\n",
    "\\end{equation*}$$\n",
    "\n",
    "    (a) What is the marginal pdf $p(x)$?\n",
    "    \n",
    "    From the lecture notes the marginal pdf of $X$ is given by: \n",
    "    \n",
    "    $$p(x) = \\int_{a}^{b} p(x, y) \\ dy$$\n",
    "    \n",
    "    Applying this to our case to get the marginal pdf $p(x)$:\n",
    "    \n",
    "    $$p(x) = \\int_{0}^{1} x + y \\ dy$$\n",
    "    \n",
    "    $$p(x) = x * \\frac{y^2}{2} \\Big|_0^1$$\n",
    "    \n",
    "    $$\\boxed{p(x) = \\frac{x}{2}, \\ \\ \\ \\ 0 \\leq x \\leq 1}$$\n",
    "    \n",
    "    <br>\n",
    "    \n",
    "    (b) What is the conditional pdf $p(y | x)$?\n",
    "    \n",
    "    Given two random variables $X$ and $Y$, the conditional pdf is given by:\n",
    "    \n",
    "    $$p(y | x) = \\frac{p(y, x)}{p(x)}$$\n",
    "    \n",
    "    We are given $p(y, x)$ (same as $p(x, y)$) and we solved for $p(x)$ in part (a). Putting it together:\n",
    "    \n",
    "    $$p(y | x) = \\frac{x + y}{\\frac{x}{2}}$$\n",
    "    \n",
    "    $$\\boxed{p(y | x) = \\frac{2(x + y)}{x}, \\ \\ \\ \\ 0 \\leq x \\leq 1, \\ \\ 0 \\leq y \\leq 1}$$\n",
    "    \n",
    "    <br>\n",
    "    \n",
    "    (c) What is the conditional expectation $E[Y | X]$?\n",
    "    \n",
    "    Given two random variables $X$ and $Y$ where $X = x$, the conditional expectation is given by: \n",
    "    \n",
    "    $$E[Y | X = x] = \\int_{-\\infty}^{\\infty} y \\ p(y|x) \\ dy$$\n",
    "    \n",
    "    Using $p(y|x)$ from part (b), we can solve for $E[Y | X = x]$:\n",
    "    \n",
    "    $$E[Y | X = x] = \\int_{0}^{1} \\frac{2y(x+y)}{x} \\ dy$$\n",
    "    \n",
    "    $$E[Y | X = x] = 2 \\int_{0}^{1} \\frac{yx+ y^2}{x} \\ dy$$\n",
    "    \n",
    "    $$E[Y | X = x] = 2 * \\frac{\\frac{xy^2}{2} + \\frac{y^3}{3}}{x} \\Big|_0^1$$\n",
    "    \n",
    "    $$E[Y | X = x] = 2 * \\frac{\\frac{x}{2} + \\frac{1}{3}}{x}$$\n",
    "    \n",
    "    $$\\boxed{E[Y | X = x] = \\frac{x + \\frac{2}{3}}{x}, \\ \\ \\ \\ 0 \\leq x \\leq 1}$$\n",
    "    \n",
    "    <br>\n",
    "\n",
    "    (d) What is the covariance $Cov(X, Y)$?\n",
    "    \n",
    "    From the lecture notes the covariance of two random variables $X$ and $Y$ is given by:\n",
    "    \n",
    "    $$Cov(X, Y) = E[XY] - E[X]E[Y]$$\n",
    "    \n",
    "    We will solve for the three parts and put it together. First, we will solve for $E[XY]$ which is given by:\n",
    "    \n",
    "    $$E[XY] = \\int_{0}^{1} \\int_{0}^{1} xy \\ p(x, y) \\ dx  \\ dy$$\n",
    "    \n",
    "    $$E[XY] = \\int_{0}^{1} \\int_{0}^{1} x^2y + xy^2 \\ dx \\ dy$$\n",
    "    \n",
    "    Integrate by x first from 0 to 1 followed by integrating by y from 0 to 1:\n",
    "    \n",
    "    $$E[XY] = \\int_{0}^{1} \\frac{y}{3} + \\frac{y^2}{2} \\ dy$$\n",
    "    \n",
    "    $$E[XY] = \\frac{1}{3}$$\n",
    "    \n",
    "    Next we will solve for $E[X]$ using $p(x)$ from part (a):\n",
    "    \n",
    "    $$E[X] = \\int_{0}^{1} x \\ p(x) \\ dx$$\n",
    "    \n",
    "    $$E[X] = \\int_{0}^{1} \\frac{x^2}{2} dx$$\n",
    "    \n",
    "    $$E[X] = \\frac{1}{6}$$\n",
    "    \n",
    "    To solve for $E[Y]$ we need $p(y)$:\n",
    "    \n",
    "    $$p(y) = \\int_{0}^{1} x + y \\ dx$$\n",
    "    \n",
    "    $$p(y) = \\frac{y}{2}$$\n",
    "    \n",
    "    Then we solve for $E[Y]$:\n",
    "    \n",
    "    $$E[Y] = \\int_{0}^{1} y \\ p(y) \\ dx$$\n",
    "    \n",
    "    $$E[Y] = \\int_{0}^{1} \\frac{y^2}{2} dx$$\n",
    "    \n",
    "    $$E[Y] = \\frac{1}{6}$$\n",
    "    \n",
    "    Finally we put it all together to get $Cov(X, Y)$:\n",
    "    \n",
    "    $$Cov(X, Y) = E[XY] - E[X]E[Y]$$\n",
    "    \n",
    "    $$Cov(X, Y) = \\frac{1}{3} - \\frac{1}{36}$$\n",
    "    \n",
    "    $$\\boxed{Cov(X, Y) = \\frac{11}{36}, \\ \\ \\ \\ 0 \\leq x \\leq 1, \\ \\ 0 \\leq y \\leq 1}$$\n",
    "    \n",
    "    <br>\n",
    "    \n",
    "3. Let $X \\sim Exp(\\lambda)$, i.e., the exponential distribution with pdf\n",
    "$p(x) = \\lambda \\exp(-\\lambda x)$. Let $Y = \\sqrt{X}$.\n",
    "\n",
    "    (a) What is the density function $p(y)$?\n",
    "    \n",
    "    To determine $p(y)$, we will transform the random variable $X$ to $Y$ using the transformation function $f(x) = \\sqrt{x}$. A requirement is $f(x)$ must be a one-to-one function, which it is. We will use the transformation technique from the lecture notes:\n",
    "    \n",
    "    $$p_y(y) = p_x(f^{-1}(y)) \\ \\mid \\frac{d}{dy} (f^{-1}(y)) \\mid$$\n",
    "    \n",
    "    Where $f^{-1}(y) = y^2$. Applying this we get:\n",
    "    \n",
    "    $$p_y(y) = p_x(y^2) \\ \\mid \\frac{d}{dy} y^2 \\mid$$\n",
    "    \n",
    "    Taking the derivative and re-arranging terms for the final result:\n",
    "    \n",
    "    $$\\boxed{p_y(y) = 2y \\lambda \\exp(-\\lambda y^2), \\ \\ y \\geq 0}$$\n",
    "\n",
    "    <br>\n",
    "    \n",
    "    (b) What is the cdf, $F(y) = P(Y \\leq y)$? Verify that $F(0) = 0$ and $F(\\infty) = 1$.\n",
    "    \n",
    "    The cdf can be defined in terms of the pdf as seen in the lecture notes:\n",
    "    \n",
    "    $$F(x) = P(X \\leq x) = \\int_{-\\infty}^{x} p(t) dt$$\n",
    "    \n",
    "    Applying this to $p(y) = 2y \\lambda \\exp(-\\lambda y^2)$ and for $y \\geq 0$:\n",
    "    \n",
    "    $$F(y) = P(Y \\leq y) = \\int_{0}^{y} 2t \\lambda \\exp(-\\lambda t^2) \\ dt$$\n",
    "    \n",
    "    Taking the definite integral from 0 to y over t:\n",
    "    \n",
    "    $$F(y) = P(Y \\leq y) = 2t \\lambda \\exp(-\\lambda t^2) \\Big|_0^y$$\n",
    "    \n",
    "    $$F(y) = P(Y \\leq y) = -exp(-\\lambda y^2) -(-exp(0)$$\n",
    "    \n",
    "    $$\\boxed{F(y) = P(Y \\leq y) = 1 - exp(-\\lambda y^2), \\ \\ y \\geq 0}$$\n",
    "    \n",
    "    Finally we can verify that $F(0) = 0$ and $F(\\infty) = 1$:\n",
    "    \n",
    "    $$\\boxed{F(0) = P(Y \\leq 0) = 1 - exp(-\\lambda * 0) = 1 - 1 = 0}$$\n",
    "    \n",
    "    $$\\boxed{F(\\infty) = P(Y \\leq \\infty) = 1 - exp(-\\lambda * \\infty) = 1 - 0 = 1}$$\n",
    "    \n",
    "    <br>\n",
    "    \n",
    "    (c) What is the quantile function $F^{-1}$?\n",
    "    \n",
    "    The quantile function $F^{-1}$ is the inverse function of the cdf ([wiki](https://en.wikipedia.org/wiki/Quantile_function)). We will start with the cdf and find its inverse by isolating $y$:\n",
    "    \n",
    "    $$p = 1 - exp(- \\lambda y^2)$$\n",
    "    \n",
    "    $$1 - p = exp(- \\lambda y^2)$$\n",
    "    \n",
    "    $$ln(1 - p) = -\\lambda y^2$$\n",
    "    \n",
    "    $$\\frac{-ln(1 - p)}{\\lambda} = y^2$$\n",
    "    \n",
    "    $$y = \\sqrt{\\frac{-ln(1 - p)}{\\lambda}}$$\n",
    "    \n",
    "    $$\\boxed{F^{-1} = \\sqrt{\\frac{-ln(1 - p)}{\\lambda}}}$$\n",
    "    \n",
    "    (d) Compute the mean, E[Y], and variance, Var(Y).\n",
    "    \n",
    "    First we will start with the mean or E[Y] which is given by:\n",
    "    \n",
    "    $$E[Y] = \\int_{0}^{\\infty} y * (2y \\ \\lambda \\ exp(-\\lambda \\ y^2)) dy$$\n",
    "    \n",
    "    We will follow the hint and do integration by parts. Choosing $u = y$, $\\frac{dv}{dx} = 2y \\ \\lambda \\ exp(- \\lambda  \\ y^2)$, $\\frac{du}{dx} = 1$, and solving for v:\n",
    "    \n",
    "    $$v = \\int 2y \\ \\lambda exp(- \\lambda \\ y^2) = -exp(-\\lambda \\ y^2)$$\n",
    "    \n",
    "    With these four values, we can solve the original integral:\n",
    "    \n",
    "    $$E[Y] = (y * -exp(-\\lambda \\ y^2))\\Big|_0^\\infty - \\int_{0}^{\\infty} -exp(-\\lambda \\ y^2) dy$$\n",
    "    \n",
    "    $$E[Y] = 0 + \\frac{\\sqrt{\\pi}}{2\\sqrt{\\lambda}}$$\n",
    "    \n",
    "    $$\\boxed{E[Y] = \\frac{\\sqrt{\\pi}}{2\\sqrt{\\lambda}}}$$\n",
    "    \n",
    "    Next we will calculate $Var(Y)$ using the formula for continuous random variables ([wiki](https://en.wikipedia.org/wiki/Variance#Continuous_random_variable)):\n",
    "    \n",
    "    $$Var(Y) = \\int y^2 \\ p(y) \\ dy \\ - E[Y]^2$$\n",
    "    \n",
    "    $$Var(Y) = \\int_{0}^{\\infty} y^2 * (2y \\ \\lambda \\ exp(-\\lambda \\ y^2))  \\ dy \\ - E[Y]^2$$\n",
    "    \n",
    "    We will use integration by parts again. Choosing $u = y^2$, $\\frac{dv}{dx} = 2y \\ \\lambda \\ exp(- \\lambda  \\ y^2)$, $\\frac{du}{dx} = 2y$, and $v = -exp(-\\lambda \\ y^2)$.\n",
    "    \n",
    "    $$Var(Y) = (y^2 * -exp(-\\lambda \\ y^2))\\Big|_0^\\infty - \\int_{0}^{\\infty} -exp(-\\lambda \\ y^2) * (2y) dy - E[Y]^2$$\n",
    "    \n",
    "    Taking the integral:\n",
    "    \n",
    "    $$Var(Y) = 0 + \\frac{1}{\\lambda} - E[Y]^2$$\n",
    "    \n",
    "    Replacing the value of $E[Y]$ found earlier in the problem:\n",
    "    \n",
    "    $$Var(Y) = \\frac{1}{\\lambda} - (\\frac{\\sqrt{\\pi}}{2\\sqrt{\\lambda}})^2$$\n",
    "    \n",
    "    $$Var(Y) = -\\frac{1}{\\lambda} - \\frac{\\pi}{4 \\lambda}$$\n",
    "    \n",
    "    \n",
    "    \n",
    "    \n",
    "    \n",
    "    "
   ]
  },
  {
   "cell_type": "code",
   "execution_count": null,
   "metadata": {
    "collapsed": true
   },
   "outputs": [],
   "source": []
  }
 ],
 "metadata": {
  "kernelspec": {
   "display_name": "Python 3",
   "language": "python",
   "name": "python3"
  },
  "language_info": {
   "codemirror_mode": {
    "name": "ipython",
    "version": 3
   },
   "file_extension": ".py",
   "mimetype": "text/x-python",
   "name": "python",
   "nbconvert_exporter": "python",
   "pygments_lexer": "ipython3",
   "version": "3.6.3"
  }
 },
 "nbformat": 4,
 "nbformat_minor": 2
}
